Clean up gensyms proofs

theories/L6_PCPS/uncurry_proto.v
@@ -1,6 +1,6 @@
 (** Uncurrying written as a guarded rewrite rule *)
 
-Require Import Coq.Strings.String.
+Require Import Coq.Strings.String Coq.Classes.Morphisms.
 Require Import Coq.NArith.BinNat Coq.PArith.BinPos Coq.Sets.Ensembles Lia.
 Require Import L6.Prototype.
 Require Import L6.cps_proto.
@@ -40,14 +40,23 @@ Definition R_e {A} (e : univD A) : Set := unit.
 Definition fresher_than (x : cps.var) (S : Ensemble cps.var) : Prop :=
   forall y, y \in S -> (x > y)%positive.
 
+Lemma fresher_than_not_In x S : fresher_than x S -> ~ x \in S.
+Proof. intros Hfresh Hin; assert (x > x)%positive by now apply Hfresh. lia. Qed.
+
 Lemma fresher_than_antimon x S1 S2 : S1 \subset S2 -> fresher_than x S2 -> fresher_than x S1.
 Proof. intros HS12 Hfresh y Hy; apply Hfresh, HS12, Hy. Qed.
 
-Lemma fresher_than_monotonic x y S : (y > x -> fresher_than x S -> fresher_than y S)%positive.
+Lemma fresher_than_monotonic x y S : (y >= x -> fresher_than x S -> fresher_than y S)%positive.
 Proof. intros Hxy Hfresh z Hz. assert (x > z)%positive by now apply Hfresh. lia. Qed.
 
 Lemma fresher_than_Union x S1 S2 : fresher_than x S1 -> fresher_than x S2 -> fresher_than x (S1 :|: S2).
 Proof. intros HS1 HS2 y Hy; destruct Hy as [y Hy|y Hy]; auto. Qed.
+
+Instance Proper_fresher_than_r : Proper (Logic.eq ==> Same_set _ ==> iff) fresher_than.
+Proof.
+  unfold Proper, "==>", fresher_than.
+  intros x y Hxy x0 y0 Hxy0; subst; split; intros Hforall dummy; now (rewrite <- Hxy0 || rewrite Hxy0).
+Qed.
 
 Definition S {A} (C : exp_c A exp_univ_exp) (e : univD A) : Set :=
   {x | fresher_than x (used_vars ![C ⟦ e ⟧])}.
@@ -121,7 +130,7 @@ Inductive uncurry_step : exp -> exp -> Prop :=
            (* Update inlining heuristic so inliner knows to inline fully saturated calls to f *)
            let s := (max (fst s) fp_numargs, (PM.set ![f] 1 (PM.set ![g] 2 (snd s)))) in
            (true, aenv, lm, s) : S_misc)
-         (* Rewrite f as a wrapper around the uncurried f1 *)
+         (* Rewrite f as a wrapper around the uncurried f1 and recur on fds *)
          (Fcons f ft (k :: fv1) (Efun (Fcons g gt gv1 (Eapp f1 ft1 (gv1 ++ fv1)) Fnil) (Eapp k kt [g]))
          (Fcons f1 ft1 (gv ++ fv) ge (Rec fds))) ⟧).
 
@@ -131,36 +140,31 @@ Fixpoint gensyms {A} (x : cps.var) (xs : list A) : cps.var * list var :=
   | _ :: xs => let '(x', xs') := gensyms (1 + x)%positive xs in (x', mk_var x :: xs')
   end.
 
-Lemma gensyms_len {A} x (xs : list A) : length (snd (gensyms x xs)) = length xs.
+Lemma gensyms_len' {A} : forall x (xs : list A) x' xs', (x', xs') = gensyms x xs -> length xs' = length xs.
 Proof.
-  revert x; induction xs; auto; intros.
-  unfold gensyms; fold @gensyms; destruct (gensyms _ _) as [x' xs'] eqn:Hxs'; simpl.
-  now erewrite <- IHxs, Hxs'.
+  intros x xs; revert x; induction xs as [|x xs IHxs]; intros x0 x' xs' Hgen; [simpl in Hgen; now inv Hgen|].
+  unfold gensyms in Hgen; fold @gensyms in Hgen.
+  destruct (gensyms (1 + x0)%positive xs) as [x'' xs''] eqn:Hx0; inv Hgen; now simpl.
+Qed.
+
+Lemma gensyms_increasing' {A} :
+  forall x (xs : list A) x' xs', (x', xs') = gensyms x xs -> 
+  forall y, List.In y xs' -> (![y] >= x)%positive.
+Proof.
+  intros x xs; revert x; induction xs as [|x xs IHxs]; intros x0 x' xs' Hgen [y] Hy;
+    [simpl in Hgen; now inv Hgen|].
+  unfold gensyms in Hgen; fold @gensyms in Hgen.
+  destruct (gensyms (1 + x0)%positive xs) as [x'' xs''] eqn:Hx0; inv Hgen; simpl.
+  simpl in Hy; destruct Hy as [H|H]; [inversion H; simpl; lia|].
+  specialize IHxs with (x := (1 + x0)%positive) (y := mk_var y).
+  rewrite Hx0 in IHxs; unfold snd in IHxs.
+  specialize (IHxs x'' xs'' eq_refl H); unfold isoBofA, Iso_var, un_var in IHxs; lia.
 Qed.
 
 Local Ltac mk_corollary parent := 
   intros x xs x' xs';
   pose (Hparent := parent _ x xs); clearbody Hparent; intros H;
   destruct (gensyms x xs); now inversion H.
-
-Corollary gensyms_len' {A} : forall x (xs : list A) x' xs', (x', xs') = gensyms x xs -> length xs' = length xs.
-Proof. mk_corollary @gensyms_len. Qed.
-
-Lemma gensyms_increasing {A} x (xs : list A) : forall y, List.In y (snd (gensyms x xs)) -> (![y] >= x)%positive.
-Proof.
-  revert x; induction xs; [now simpl|intros x [y] Hy].
-  unfold gensyms in Hy; fold @gensyms in Hy.
-  destruct (gensyms _ _) as [x' xs'] eqn:Hxs'.
-  simpl in Hy; destruct Hy as [H|H]; [inversion H; simpl; lia|].
-  specialize (IHxs (1 + x)%positive (mk_var y)).
-  rewrite Hxs' in IHxs; unfold snd in IHxs.
-  specialize (IHxs H); lia.
-Qed.
-
-Corollary gensyms_increasing' {A} :
-  forall x (xs : list A) x' xs', (x', xs') = gensyms x xs -> 
-  forall y, List.In y xs' -> (![y] >= x)%positive.
-Proof. mk_corollary @gensyms_increasing. Qed.
 
 Lemma gensyms_upper {A} x (xs : list A) :
   (fst (gensyms x xs) >= x)%positive /\
@@ -194,13 +198,14 @@ Proof.
   destruct (gensyms _ _) as [x' xs'] eqn:Hxs'; unfold snd.
   specialize (IHxs (1 + x)%positive); rewrite Hxs' in IHxs; unfold snd in IHxs.
   constructor; [|auto].
-  pose (Hinc := gensyms_increasing (1 + x)%positive xs); clearbody Hinc.
+  pose (Hinc := gensyms_increasing' (1 + x)%positive xs); clearbody Hinc.
   rewrite Hxs' in Hinc; unfold snd in Hinc.
   remember (snd (gensyms (1 + x)%positive xs)) as ys; clear - Hinc.
   induction xs'; auto.
-  intros [|Hin_ys]; [|apply IHxs'; auto; intros; apply Hinc; now right].
+  specialize (Hinc x' (a :: xs')).
+  intros [|Hin_ys]; [|apply IHxs'; auto; intros; apply Hinc; auto; now right].
   assert (Hxa : In (mk_var x) (a :: xs')) by now left.
-  specialize (Hinc (mk_var x) Hxa); unfold isoBofA, Iso_var, un_var in Hinc; lia.
+  specialize (Hinc eq_refl (mk_var x) Hxa); unfold isoBofA, Iso_var, un_var in Hinc; lia.
 Qed.
 
 Corollary gensyms_NoDup' {A} : forall x (xs : list A) x' xs', (x', xs') = gensyms x xs -> NoDup xs'.
@@ -260,13 +265,36 @@ Proof.
   lia.
 Qed.
 
+Lemma gensyms_spec {A} x S (xs : list A) x' xs' : 
+  fresher_than x S ->
+  (x', xs') = gensyms x xs ->
+  fresh_copies S xs' /\ fresher_than x' (S :|: FromList ![xs']) /\ length xs' = length xs.
+Proof.
+  intros Hfresh Hgen; unfold fresh_copies; split; [split|split].
+  - show_Disjoint arb Harbx Harby.
+    unfold Ensembles.In, FromList in Harby; apply (in_map mk_var) in Harby.
+    simpl in Harby; normalize_roundtrips.
+    assert (x > arb)%positive by now apply Hfresh.
+    assert (![mk_var arb] >= x)%positive by (eapply gensyms_increasing'; eauto).
+    simpl in *; lia.
+  - eapply gensyms_NoDup'; eauto.
+  - intros y Hy; destruct Hy as [y Hy|y Hy].
+    + assert (x > y)%positive by now apply Hfresh.
+      assert (x' >= x)%positive by (eapply gensyms_upper1; eauto); lia.
+    + unfold Ensembles.In, FromList in Hy; apply (in_map mk_var) in Hy.
+      simpl in Hy; normalize_roundtrips.
+      change y with ![mk_var y].
+      eapply gensyms_upper2; eauto.
+  - eapply gensyms_len'; eauto.
+Qed.
+
 Lemma bool_true_false b : b = false -> b <> true. Proof. now destruct b. Qed.
 
 Local Ltac clearpose H x e :=
   pose (x := e); assert (H : x = e) by (subst x; reflexivity); clearbody x.
 
 (* Uncurrying as a recursive function *)
-Definition rw_cp : rewriter exp_univ_exp uncurry_step R_misc S_misc (@delay_t) (@R_C) (@R_e) (@S).
+Definition uncurry_proto : rewriter exp_univ_exp uncurry_step R_misc S_misc (@delay_t) (@R_C) (@R_e) (@S).
 Proof.
   mk_rw;
     (* This particular rewriter's delayed computation is just the identity function,
@@ -302,50 +330,16 @@ Proof.
     clearpose Hxfv1 xfv1 (gensyms next_x0 fv); destruct xfv1 as [next_x1 fv1].
     clearpose Hf1 f1 next_x1.
     (* Prove that all the above code actually satisfies the side condition *)
-    assert (NoDup gv1) by (eapply gensyms_NoDup'; eassumption).
-    assert (NoDup fv1) by (eapply gensyms_NoDup'; eassumption).
-    assert (length gv1 = length gv) by (eapply gensyms_len'; eassumption).
-    assert (length fv1 = length fv) by (eapply gensyms_len'; eassumption).
     assert (next_x0 >= next_x)%positive by (eapply gensyms_upper1; eassumption).
     assert (next_x1 >= next_x0)%positive by (eapply gensyms_upper1; eassumption).
-    assert (Disjoint _ (FromList ![gv1]) (FromList ![fv1])) by (eapply gensyms_disjoint; eassumption).
+    edestruct (@gensyms_spec var) as [Hgv_copies [Hfresh_gv Hgv_len]]; try exact Hxgv1; [eassumption|].
+    edestruct (@gensyms_spec var) as [Hfv_copies [Hfresh_fv Hfv_len]]; try exact Hxfv1; [eassumption|].
     eapply success with (f1 := mk_var f1) (fv1 := fv1) (gv1 := gv1) (next_x := (next_x1 + 1)%positive);
-      repeat match goal with
-      | |- _ /\ _ => split
-      | |- fresh_copies _ _ => split
-      | |- Disjoint _ (_ :|: _) _ => apply Union_Disjoint_l
-      end;
-      try solve [reflexivity|assumption|subst;reflexivity].
-    + eapply gensyms_list_fresher; [| |eassumption]; try eassumption; lia.
-    + eapply gensyms_list_fresher; [| |eassumption]; try eassumption; lia.
-    + match goal with |- ~ _ \in _ => rewrite <- Disjoint_Singleton_In; [|auto with Decidable_DB] end.
-      repeat match goal with |- Disjoint _ (_ :|: _) _ => apply Union_Disjoint_l end.
-      * subst f1; simpl; show_Disjoint arb Harbx Harby.
-        assert (next_x > arb)%positive by now apply Hnext_x.
-        inversion Harby; lia.
-      * show_Disjoint arb Harbx Harby; simpl in Harby.
-        unfold Ensembles.In, FromList in Harbx; apply (in_map mk_var) in Harbx.
-        simpl in Harbx; normalize_roundtrips.
-        assert (Harb0 : (next_x0 > ![mk_var arb])%positive) by (eapply gensyms_upper2; eauto).
-        simpl in Harb0; inv Harby.
-        lia. (* arb >= next_0 >= next_x > arb *)
-      * show_Disjoint arb Harbx Harby.
-        simpl in Harby; inv Harby.
-        unfold Ensembles.In, FromList in Harbx; apply (in_map mk_var) in Harbx.
-        simpl in Harbx; normalize_roundtrips.
-        assert (Harb : (arb > ![mk_var arb])%positive) by (eapply gensyms_upper2; eauto).
-        simpl in Harb; lia.
-    + repeat match goal with |- fresher_than _ (_ :|: _) => apply fresher_than_Union end.
-      * eapply fresher_than_monotonic; eauto; lia.
-      * intros z Hz; unfold Ensembles.In, FromList in Hz; apply (in_map mk_var) in Hz.
-        simpl in Hz; normalize_roundtrips.
-        assert (Hz0 : (next_x0 > ![mk_var z])%positive) by (eapply gensyms_upper2; eauto).
-        simpl in Hz0; lia.
-      * intros z Hz; unfold Ensembles.In, FromList in Hz; apply (in_map mk_var) in Hz.
-        simpl in Hz; normalize_roundtrips.
-        assert (Hz0 : (next_x1 > ![mk_var z])%positive) by (eapply gensyms_upper2; eauto).
-        simpl in Hz0; lia.
-      * simpl; intros f1' Hf1'; inversion Hf1'; lia.
+      repeat match goal with |- _ /\ _ => split end;
+      try solve [reflexivity|eassumption|subst;reflexivity].
+    + apply fresher_than_not_In; subst f1; exact Hfresh_fv.
+    + apply fresher_than_Union; [|subst; simpl; intros y Hy; inversion Hy; lia].
+      eapply fresher_than_monotonic; eauto; lia.
     + left; exact I. (* TODO replace with actual proof *)
     + destruct (Maps.PTree.get _ _) as [[|]|] eqn:Hget'; [reflexivity|inversion Huncurried..].
   (* Obligation 2 of 2: explain how to maintain fresh name invariant across edit *)
@@ -363,3 +357,5 @@ Proof.
     repeat rewrite strip_vars_app; repeat normalize_sets.
     intros arbitrary; repeat rewrite In_or_Iff_Union; tauto.
 Defined.
+
+Recursive Extraction uncurry_proto.
